more erasure of ghost lambdas

src/extraction/codegen.fs
@@ -300,12 +300,6 @@ let rec doc_of_mltype' (currentModule : mlsymbol) (outer : level) (ty : mlty) =
         let d2 = doc_of_mltype currentModule (t_prio_fun, Right) t2 in
         maybe_paren outer t_prio_fun (hbox (reduce1 [d1; text " -> "; d2]))
 
-    | MLTY_App (t1, t2) ->
-        let d1 = doc_of_mltype currentModule (t_prio_fun, Left ) t1 in
-        let d2 = doc_of_mltype currentModule (t_prio_fun, Right) t2 in
-
-        maybe_paren outer t_prio_fun (hbox (reduce1 [d2; text " "; d1]))
-
     | MLTY_Top ->
       if Util.codegen_fsharp()
       then text "obj"
