src/extraction/ml-syntax.fs
@@ -35,10 +35,9 @@ type e_tag =
 
 type mlty =
 | MLTY_Var   of mlident
-| MLTY_Fun   of mlty * e_tag * mlty //t -> MayErase t', or  t -> Keep t'
+| MLTY_Fun   of mlty * e_tag * mlty 
 | MLTY_Named of list<mlty> * mlpath
 | MLTY_Tuple of list<mlty>
-| MLTY_App   of mlty * mlty         //Why do we have a type-application form? The only applications in ML are of named constructors
 | MLTY_Top
 
 type mltyscheme = mlidents * mlty   //forall a1..an. t  (the list of binders can be empty)
