examples/bug-reports/bug086.fst
@@ -35,3 +35,15 @@ let repr_bytes2 n =
       else if n < 281474976710656 then 6
       else if n < 72057594037927936 then 7
       else 8
+
+
+val grepr_bytes : nat -> nat -> GTot nat
+let grepr_bytes n _ =
+      if n < 256 then 1
+      else if n < 65536 then 2
+      else if n < 16777216 then 3
+      else if n < 4294967296 then 4
+      else if n < 1099511627776 then 5
+      else if n < 281474976710656 then 6
+      else if n < 72057594037927936 then 7
+      else 8
